![[MTH1002M_Calculus_Practical_2.pdf]]
### Question 1
$$
f(x)=\frac{2x}{3x^2+1}\implies f(-x)=\frac{-2x}{3x^2+1}:\text{odd}
$$
$$
f(x)=\frac{3x^2}{3x^4+4}\implies f(-x)=\frac{3x^2}{3x^4+4}:\text{even}
$$
$$
f(x)=1+x^3-x^5\implies f(-x)=1-x^3+x^5:\text{neither}
$$
$$
f(x)=\ln(2x^6-x^4+2)\implies f(-x)=\ln(2x^6-x^4+2):\text{even}
$$
$$
g(t)=\frac{2t^3+t-1}{3t^2+5}\implies f(-x)=\frac{-2t^3-t-1}{3t^2+5}:\text{neither}
$$
$$
h(x)=\frac{ax^3+bx}{cx^2+d}\implies f(-x)=\frac{-ax^3-bx}{cx^2+d}:\text{odd}
$$
### Question 2
Prove $\cosh^2 x - \sinh^2 x = 1$:
$$
\cosh^2 x - \sinh^2 x =1:LHS=(\frac{e^x+e^{-x}}{2})^2-(\frac{e^x-e^{-x}}{2})^2,RHS=1
$$
$$
\implies LHS=\frac{e^{2x}+2+e^{-2x}}{4}-\frac{e^{2x}-2+e^{-2x}}{4}
$$
$$
\implies LHS=\frac{4}{4},RHS=1\therefore LHS=RHS\space\blacksquare
$$
Hence, prove that $\text{sech}^2 x = 1 - \tanh^2 x$ and $\text{cosech}^2 x = \coth^2 x - 1$:
$$
\frac{\cosh^2 x}{\cosh^2 x} - \frac{\sinh^2 x}{\cosh^2 x} = \frac{1}{\cosh^2 x}
$$
$$
\implies1-\tanh^2 x=\text{sech}^2 x\space\blacksquare
$$
$$
\frac{\cosh^2 x}{\sinh^2 x} - \frac{\sinh^2 x}{\sinh^2 x} = \frac{1}{\sinh^2 x}
$$
$$
\implies \coth^2x-1=\text{cosech}^2x\space\blacksquare
$$
### Question 3
$i^2=-1$
$i^3=-i$
$i^4=1$
$i^5=i$
$i^{100}=1$
$i^{505}=i$
$i^{-1}=\frac{1}{i}=-i$
$i^{-7}=-\frac{1}{i}=i$
### Question 4
$z_1=-2+i,z_2=1-3i$, such that:

$\Re(z_1)=-2$
$\Im(z_1)=1$

$\Re(z_2)=1$
$\Im(z_2)=-3$

$|z_1|=\sqrt{(-2)^2+(1)^2}=\sqrt{5}$
$|z_2|=\sqrt{(1)^2+(-3)^2}=\sqrt{10}$

$\angle(z_1)=-\tan^{-1}(\frac{1}{2})$
$\angle(z_2)=-\tan^{-1}(3)=-\frac{\pi}{4}$
### Question 5
$z_1=3-2i,z_2=1+4i$, such that

$z_1+z_2=4+2i$
$z_1-z_2=2-6i$

$z_1z_2=11+10i$
$\frac{z_1}{z_2}=-\frac{5+14i}{17}=-\frac{5}{17}-\frac{14}{17}i$

$\frac{z_2}{z_1}=\frac{-5+14i}{13}=-\frac{5}{13}+\frac{14}{13}i$
$\bar{z_1}\bar{z_2}=(3+2i)(1-4i)=11-10i$
### Question 6
$1+i : (r,\theta) = (\sqrt{2},\frac{\pi}{4})$
$-1+i : (r,\theta) = (\sqrt{2},\frac{3\pi}{4})$
$-1-i : (r,\theta) = (\sqrt{2},\frac{5\pi}{4})$
$\sqrt{3}+i:(r,\theta) = (2,\frac{\pi}{6})$
$\sqrt{3}-i:(r,\theta) = (2,\frac{11\pi}{6})$
$-\sqrt{3}-i:(r,\theta) = (2,\frac{4\pi}{3})$
### Question 7
$$\frac{1+i}{i(2-3i)}+\frac{2}{i}=\frac{i(1+i)+2i(2-3i)}{3i-2}=\frac{5i+5}{3i-2}$$
$$
\implies\frac{5i+5}{3i-2}=\frac{25i-5}{13}=-\frac{5}{13}+\frac{25}{13}i
$$

$$\frac{1}{3+2i}+\frac{1}{2-i}=\frac{41}{65}+\frac{3}{65}i$$
### Question 8
Show that the product of two odd functions, $f(x)$ and $g(x)$, is always an even function.

Let $f(x),g(x)$ be such that $f(-x)=-f(x),g(-x)=-g(x)$.
Thus, if we take the product of the two functions: $h(x)=f(x)g(x)$, prove that $h(-x)=h(x)$.
$$
h(-x)=f(-x)\cdot g(-x)=-f(x)\cdot-g(x)=f(x)\cdot g(x)=h(x)
$$
$$
\therefore h(-x)=h(x)\space\blacksquare
$$
