Rough work for [[MTH1008 Personal Tutoring]] on [[2023-10-30]]
$$
y=\ln\left(\frac{\cosh x-1}{\cosh x+1}\right)=\ln(\cosh x-1)-\ln(\cosh x+1)
$$
$$
\implies\frac{dy}{dx}=\frac{\sinh x}{\cosh x - 1}-\frac{\sinh x}{\cosh x + 1}
$$
$$
\implies\frac{dy}{dx}=\frac{\sinh x(\cosh x+1)-\sinh x(\cosh x - 1)}{\sinh^2 x}
$$
$$
\implies\frac{dy}{dx}=\frac{2\sinh x}{\sinh^2 x}
$$
$$
\implies\frac{dy}{dx}=2\csc x
$$
___
$$
1+\frac{3}{4x-8}-\frac{3}{4x+8}\implies1+\frac{3(4x+8)-3(4x-8)}{16x^2-64}
$$
$$
\implies1+\frac{48}{16x^2-64}\implies\frac{16x^2-16}{16x^2-64}\implies\frac{x^2-1}{x^2-4}
$$
___
$$
y=\ln(x^2\sqrt{1-x^2})\implies y=2\ln x+\frac{1}{2}\ln(1-x^2)
$$
$$
\frac{dy}{dx}=\frac{2}{x}-\frac{x}{1-x^2}\implies\frac{dy}{dx}=\frac{2(1-x^2)-x^2}{x(1-x^2)}
$$
$$
\implies\frac{dy}{dx}=\frac{2-3x^2}{x(1-x^2)}
$$
___
$$
y = \frac{e^{2x}\cdot\ln x}{(x-3)^3}
$$
$$
\implies\ln y=\ln(e^{2x}\cdot\ln x)-3\ln(x-3)
$$
$$
\implies \ln y = 2x+\ln(\ln x)-3\ln(x-3)
$$
$$
\implies\frac{1}{y}\cdot\frac{dy}{dx}=2+\frac{1}{x\ln x}-\frac{3}{x-3}
$$
$$
\frac{dy}{dx}=\left(\frac{e^{2x}\cdot\ln x}{(x-3)^3}\right)\cdot\left(2+\frac{1}{x\ln x}-\frac{3}{x-3}\right)
$$
___
Find an expression for the slope on the lower-half of the circle:
$$
x^2+y^2=25\implies2x+2y\frac{dy}{dx}=0
$$
$$
\frac{dy}{dx}=-\frac{x}{y}:y=-\sqrt{25-x^2}\implies\frac{x}{\sqrt{25-x^2}}
$$
___
Find the slope of a general point of the expression
$$
\frac{x^2}{a^2}+\frac{y^2}{b^2}=1
$$
$$
\implies\frac{2x}{a^2}+\frac{2y}{b^2}\frac{dy}{dx}=0
$$
$$
\implies\frac{dy}{dx}=-\frac{x\cdot b^2}{y\cdot a^2}
$$
___
