![[MTH1002M_Calculus_Practical_1.pdf]]
### Question 1
The domain and range of the functions in question 1 are as follows, respectively:
$$
\text{Domain: }\mathbb{R}
,\space\text{Range: }[0,\infty)
$$
$$
\text{Domain: }\mathbb{R}
,\space\text{Range: }\mathbb{R}
$$
$$
\text{Domain: }[-\sqrt{5},\sqrt{5}]
,\space\text{Range: }[0,\sqrt{5}]
$$
$$
\text{Domain: }[0,\infty)
,\space\text{Range: }[0,\infty)
$$
$$
\text{Domain: }(-\infty,0)\cup(0,\infty)
,\space\text{Range: }(-\infty,0)\cup(0,\infty)
$$
$$
\text{Domain: }(-\infty,0)\cup(0,\infty)
,\space\text{Range: }(0,\infty)
$$
$$
\text{Domain: }(-\infty,3)\cup(3,\infty)
,\space\text{Range: }(-\infty,0)\cup(0,\infty)
$$
$$
\text{Domain: }(-2,2)
,\space\text{Range: }[\frac{1}{2},\infty)
$$
$$
\text{Domain: }(-\infty,a]
,\space\text{Range: }[0,\infty)
$$
$$
\text{Domain: }(-\infty,b)\cup(b,\infty)
,\space\text{Range: }(0,\infty)
$$
### Question 2
The degree of the respective polynomials shown in the question would be: 1, 3, 7, 0.
### Question 3
*Complete at home with my drawing tablet*
![[Cos graph.excalidraw]]
### Question 4
*Complete at home with my drawing tablet*
### Question 5
*Complete at home with my drawing tablet*
Yes, in the lecture we proposed splitting the function into two functions for the top and the bottom - thus here we can split the function in the two sides: $x^2+y^2=r^2\implies$ 
### Question 6
The function would be equal to $\frac{0}{0}=\text{undefined}$, thus $x=-2$ shouldn't be included in the domain.
### Question 7
The function of $\cos$ as a power series is as follows:
$$
\cos x = 1 - \frac{x^2}{2!} + \frac{x^4}{4!} - \ldots
$$
Differentiating that gives the function of $-\sin$ as shown below:
$$
\frac{d}{dx}(1 - \frac{x^2}{2!} + \frac{x^4}{4!} - \ldots)=-x+\frac{x^3}{3!}-\ldots=-(x-\frac{x^3}{3!}+\ldots)=-\sin x
$$
### Question 8
$\sin^2 x + \cos^2 x \equiv 1\implies \frac{\sin^2 x}{\sin^2 x} + \frac{\cos^2}{\sin^2 x} x \equiv \frac{1}{\sin^2 x}\implies1+\cot^2 x\equiv\csc^2 x$
Which is equivalent to the required result.

To show that $\frac{2\sin x}{1-\cos x}-\frac{2\cos x}{\sin x}\equiv 2\csc x$, it is a bit more involved:
$\sin^2 x + \cos^2 x \equiv 1$
$\implies 2\sin^2 x + 2\cos^2 x \equiv 2$
$\implies 2\sin^2 x - 2\cos x+2\cos^2 x + 2\cos x\equiv2$
$\implies 2\sin^2 x -(2\cos x)(1-\cos x)\equiv2-2\cos x$
$\implies \frac{2\sin^2 x}{1-\cos x}-2\cos x\equiv2$
### Question 9
As $n$ increases, the gradient change between the two asymptotes is quicker, slowly tending towards perfectly meeting the asymptotes looking like a right-angle. This is explainable through the derivative of the function (which represents the gradient) similarly growing in order (thus gradient changes occur exponentially quickly), so by about $n=11$ it already looks like a right angle.
### Question 10
$$
\cos x = 1 - \frac{x^2}{2!} + \frac{x^4}{4!} - \ldots=\sum_{n=0}^{\infty}\frac{(-1)^nx^{2n}}{(2n)!}
$$
$$
\sin x = x - \frac{x^3}{3!} + \frac{x^5}{5!} - \ldots =\sum_{n=0}^{\infty}\frac{(-1)^nx^{2n+1}}{(2n+1)!}
$$
